MinWeightBasis.thy
@@ -1,5 +1,5 @@
 theory MinWeightBasis
-  imports "../../Sepreftime" "../../Refine_Foreach"
+  imports "NREST.NREST" "SeprefTime.Refine_Foreach"
     "List-Index.List_Index" Matroids.Matroid     
 begin
   
