Union_Find_Time_alpha_verification.thy
@@ -1,7 +1,12 @@
 theory Union_Find_Time_alpha_verification
-  imports Union_Find_Time_alpha_abstract_analysis Union_Find_Time_alpha_fix
+  imports
+    Union_Find_Time_alpha_abstract_analysis Union_Find_Time_alpha_fix
 begin
 
+(* TODO: MOVE *)
+
+  lemma per_union_impl: "(i,j)\<in>R \<Longrightarrow> (i,j)\<in>per_union R a b"
+    by (auto simp: per_union_def)
 
 subsubsection\<open>uf_init_lemmas\<close>
 
@@ -377,34 +382,4 @@ lemma uf_union_rule: "\<lbrakk>i\<in>Domain R; j\<in> Domain R\<rbrakk>
   done 
 
 
-interpretation UnionFind_Impl is_uf uf_init uf_init_time uf_cmp uf_cmp_time uf_union uf_union_time
-proof (unfold_locales, goal_cases)
-case (1 t x' x)
-  show ?case
-    unfolding PR_CONST_def mop_per_init_def apply simp
-    apply(rule extract_cost_otherway'[OF _ uf_init_rule', where Cost_lb="uf_init_time x"])
-      apply (sep_auto simp: per_init'_def hn_ctxt_def pure_def)+
-    using 1 by simp
-next
-  case (2 t R' R a' a b' b)
-   show ?case 
-    unfolding PR_CONST_def mop_per_compare_def apply simp
-    apply(rule extract_cost_otherway'[OF _ uf_cmp_rule_abstract, where Cost_lb="(uf_cmp_time (card (Domain R')))"])
-      apply (sep_auto simp: per_init'_def hn_ctxt_def pure_def)+
-    using 2 by simp
-next
-  case (3  t R' R a' a b' b)
-   show ?case 
-    unfolding PR_CONST_def mop_per_union_def apply simp
-    apply(rule extract_cost_otherway'[OF _ uf_union_rule, where Cost_lb="(uf_union_time (card (Domain R')))"])
-        apply (sep_auto simp: per_init'_def hn_ctxt_def pure_def)+
-    subgoal using 3 by simp
-      apply (sep_auto simp: per_init'_def hn_ctxt_def pure_def)+
-    subgoal using 3 by simp
-      apply (sep_auto simp: per_init'_def hn_ctxt_def pure_def invalid_assn_def)+
-    using 3 by simp
-qed
-
-thy_deps(Partial_Equivalence_Relation|Sepref|Asymptotics_1D|InverseNatNat)
-unused_thms
 end
